src/Iris/Std.lean
@@ -1,6 +1,5 @@
 import Iris.Std.Classes
 import Iris.Std.Expr
-import Iris.Std.Heap
 import Iris.Std.HeapInstances
 import Iris.Std.Infinite
 import Iris.Std.Nat
